examples/permanent.v
@@ -27,7 +27,7 @@ Definition server : val := rec: "loop" "c" "l" "sk" :=
   (* Receive request from the network *)
   let: <> := recv "c" in
   (* Sign message *)
-  let: "reply" := sign (Tag nroot) "sk" (! "l") in
+  let: "reply" := sign "sk" (Tag nroot) (! "l") in
   send "c" "reply";;
   "loop" "c" "l" "sk".
 
@@ -39,7 +39,7 @@ Definition client : val := λ: "c" "vk",
     (* Wait for response *)
     let: "reply" := recv "c" in
     (* Check signature *)
-    bind: "value" := verify (Tag nroot) "vk" "reply" in
+    bind: "value" := verify "vk" (Tag nroot) "reply" in
     SOME "value"
   ).
 
